verify/Individual33.v
@@ -1,4 +1,6 @@
 From BusyCoq Require Export Individual BB33.
+Require Import Ascii.
+Require Import String.
 
 Module Individual33 := Individual BB33.
 Export Individual33.
@@ -21,3 +23,101 @@ Notation "l '{{C}}>'  r" := (l {{C}}> r) (at level 30).
 Notation "l '<{{A}}' r" := (l <{{A}} r) (at level 30).
 Notation "l '<{{B}}' r" := (l <{{B}} r) (at level 30).
 Notation "l '<{{C}}' r" := (l <{{C}} r) (at level 30).
+
+
+Definition Sym_from_char(x:ascii):option Sym :=
+match x with
+| "0"%char => Some S0
+| "1"%char => Some S1
+| "2"%char => Some S2
+| _ => None
+end.
+
+Definition dir_from_char(x:ascii):option dir :=
+match x with
+| "L"%char => Some L
+| "R"%char => Some R
+| _ => None
+end.
+
+Definition Q_from_char(x:ascii):option Q :=
+match x with
+| "A"%char => Some A
+| "B"%char => Some B
+| "C"%char => Some C
+| _ => None
+end.
+
+Definition trans_from_char(c0 c1 c2:ascii):option (Sym * dir * Q) :=
+  match (Sym_from_char c0),(dir_from_char c1),(Q_from_char c2) with
+  | Some o, Some d, Some s => Some (o,d,s)
+  | _,_,_ => None
+  end.
+
+Definition trans_from_str(x:string): string*(option (Sym * dir * Q)) :=
+match x with
+| (String c0 (String c1 (String c2 x0))) =>
+  (x0,trans_from_char c0 c1 c2)
+| _ => (x,None)
+end.
+
+Definition skip_sep(x:string): string :=
+match x with
+| String ("_"%char) x0 => x0
+| _ => x
+end.
+
+Definition Q_from_str(x:string) :=
+  let (x,A0):=trans_from_str x in
+  let (x,A1):=trans_from_str x in
+  let (x,A2):=trans_from_str x in
+  let x:=skip_sep x in
+  (x,A0,A1,A2).
+
+Definition TM_from_str(x:string):TM :=
+  let '(x,A0,A1,A2):=Q_from_str x in
+  let '(x,B0,B1,B2):=Q_from_str x in
+  let '(x,C0,C1,C2):=Q_from_str x in
+  fun '(q,s) =>
+  match q,s with
+  | A,0 => A0  | A,1 => A1 | A,2 => A2
+  | B,0 => B0  | B,1 => B1 | B,2 => B2
+  | C,0 => C0  | C,1 => C1 | C,2 => C2
+  end.
+
+Definition Sym_to_str(x:Sym):string :=
+match x with
+| S0 => "0"
+| S1 => "1"
+| S2 => "2"
+end.
+
+Definition dir_to_str(x:dir):string :=
+match x with
+| L => "L"
+| R => "R"
+end.
+
+Definition Q_to_str(x:Q):string :=
+match x with
+| A => "A"
+| B => "B"
+| C => "C"
+end.
+
+Definition Trans_to_str(x:option (Sym*dir*Q)):string :=
+match x with
+| None => "---"
+| Some (o,d,s) => (Sym_to_str o) ++ (dir_to_str d) ++ (Q_to_str s)
+end.
+
+Definition TM_Q_to_str(tm:TM)(q:Q):string :=
+  (Trans_to_str (tm (q,S0))) ++
+  (Trans_to_str (tm (q,S1))) ++
+  (Trans_to_str (tm (q,S2))).
+
+Definition TM_to_str(tm:TM):string :=
+  (TM_Q_to_str tm A) ++ "_" ++
+  (TM_Q_to_str tm B) ++ "_" ++
+  (TM_Q_to_str tm C).
+
