verify/Inductive33.v
@@ -1,0 +1,13 @@
+Require Export String.
+Require Export NArith.
+From BusyCoq Require Export Individual33.
+From BusyCoq Require Import Inductive.
+
+Module Inductive33 := Inductive BB33.
+Export Inductive33.
+
+Open Scope string.
+
+
+
+
