verify/RRBA3x3v2.v
@@ -1,0 +1,35 @@
+From BusyCoq Require Import Individual33.
+From BusyCoq Require Import RRBA.
+Module RRBA33 := RRBA BB33.
+Export RRBA33.
+Require Import NArith.
+Require Import String.
+
+
+Ltac solve_loop2'' min_b n_skip k T :=
+  match goal with
+  | |- ~halts (TM_from_str ?x) c0 =>
+    idtac x;
+    apply (decide_loop2_spec' _ (min_b,16%nat) n_skip k T);
+    native_cast_no_check (eq_refl true)
+  end.
+Ltac solve_loop2' n_skip k T := solve_loop2'' O n_skip k T.
+Ltac solve_loop2 k T := solve_loop2' O k T.
+
+Close Scope sym.
+
+Lemma tm1: ~halts (TM_from_str "1RB2LA0LA_1LA2RC0RC_---2RB0RB") c0.
+Proof. solve_loop2 6 2000%N. Time Qed.
+
+Lemma tm2: ~halts (TM_from_str "1RB1LB0LB_2LA1RB0RC_---1RC2RB") c0.
+Proof. solve_loop2 6 2000%N. Time Qed.
+
+Lemma tm3: ~halts (TM_from_str "1RB1LA0LA_2LA0RC2RC_---0RB2RB") c0.
+Proof. solve_loop2 6 2000%N. Time Qed.
+
+Lemma tm4: ~halts (TM_from_str "1RB0LC2LA_2LC0RA2RA_---1LA2LC") c0.
+Proof. solve_loop2 6 2000%N. Time Qed.
+
+Lemma tm5: ~halts (TM_from_str "1RB2LA0RC_1LA0LA1RA_---1LB0RB") c0.
+Proof. solve_loop2 9 6000%N. Time Qed.
+
