verify/RWLAcc33.v
@@ -1,0 +1,12 @@
+Require Export String.
+Require Export NArith.
+From BusyCoq Require Export Individual33.
+From BusyCoq Require Export RWLAcc.
+
+Module RWLAcc33 := RWLAcc BB33.
+Export RWLAcc33.
+
+Open Scope string.
+
+
+
