verify/RWLAcc3x3Haltv1.v
@@ -1,0 +1,144 @@
+From BusyCoq Require Import RWLAcc33.
+
+Open Scope list.
+
+Ltac native_check_eq :=
+match goal with
+| |- _ = ?a => native_cast_no_check (eq_refl a)
+end.
+
+Ltac solve_halt' bsz bmaxT use_acc mnc T :=
+  eapply (decide_halt_spec _ bsz bmaxT use_acc mnc T);
+  native_check_eq.
+
+Ltac solve_halt'' bsz use_acc :=
+  match goal with
+  | |- halts_at_trans (TM_from_str ?x) c0 _ =>
+    idtac x;
+    solve_halt' bsz 3200 use_acc 2%N 100000000%N
+  end.
+
+Fixpoint get_len(ls:RWL):N :=
+match ls with
+| (w,_,n)::t => (N.of_nat (List.length w) * n + get_len t)%N
+| _ => N0
+end.
+
+Definition chk tm bsz use_acc T :=
+  match RWL_steps tm bsz 3200 use_acc 2%N T with
+  | inr x => inr x
+  | inl (c1,c2,l,r) =>
+    let '(l0,r0,_,_):=c2 in
+    inl (get_len l0 + get_len r0)%N
+  end.
+
+Ltac test_bsz bsz use_acc T :=
+  match goal with
+  | |- halts_at_trans (?x) c0 _ =>
+    pose (chk x bsz use_acc T) as v;
+    time native_compute in v;
+    match goal with
+    | _ := ?x : _ |- _ => idtac x
+    end;
+    clear v
+  end.
+
+Ltac test_bszs use_acc T :=
+  test_bsz 1%nat use_acc T;
+  test_bsz 2 use_acc T;
+  test_bsz 3 use_acc T;
+  test_bsz 4 use_acc T;
+  test_bsz 5 use_acc T;
+  test_bsz 6 use_acc T;
+  test_bsz 7 use_acc T;
+  test_bsz 8 use_acc T.
+
+Fixpoint sel_bsz_0 tm bsz n T cur_bsz cur_sz :=
+  match (chk tm bsz true T) with
+  | inl x =>
+    let (nxt_bsz,nxt_sz) := (if cur_sz <? x then (bsz,x) else (cur_bsz,cur_sz))%N in
+    match n with
+    | S n0 => sel_bsz_0 tm (S bsz) n0 T nxt_bsz nxt_sz
+    | O => cur_bsz
+    end
+  | inr x => bsz
+  end.
+
+Definition sel_bsz tm := sel_bsz_0 tm 1%nat 12 (10^4)%N 1 N0.
+
+Ltac solve_halt :=
+  match goal with
+  | |- halts_at_trans (?tm) c0 _ =>
+    solve_halt'' (sel_bsz tm) true
+  end.
+
+
+Lemma tm1: halts_at_trans (TM_from_str "1RB2LA1LC_0LA2RB1LB_---1RA1RC") c0 (C,0).
+Proof. solve_halt. Time Qed.
+
+Lemma tm2: halts_at_trans (TM_from_str "1RB1LB2LA_1LA1RC---_0LA2RC1LC") c0 (B,2).
+Proof. solve_halt. Time Qed.
+
+Lemma tm3: halts_at_trans (TM_from_str "1RB2RC1LA_2LA1RB---_2RB2RA1LC") c0 (B,2).
+Proof. solve_halt. Time Qed.
+
+Lemma tm4: halts_at_trans (TM_from_str "1RB2RA1LA_2LA2LB2RC_---2RB1RB") c0 (C,0).
+Proof. solve_halt. Time Qed.
+
+Lemma tm5: halts_at_trans (TM_from_str "1RB2LA1LA_2LA1RC2RB_---0LC0RA") c0 (C,0).
+Proof. solve_halt. Time Qed.
+
+Lemma tm6: halts_at_trans (TM_from_str "1RB1LA2LC_2LA2RB1RB_---0LB0RC") c0 (C,0).
+Proof. solve_halt. Time Qed.
+
+Lemma tm7: halts_at_trans (TM_from_str "1RB1LA2LA_1LB1RC---_1LA2RC1LC") c0 (B,2).
+Proof. solve_halt. Time Qed.
+
+Lemma tm8: halts_at_trans (TM_from_str "1RB2LA1RA_1LB1LA2RC_---1LC2RB") c0 (C,0).
+Proof. solve_halt. Time Qed.
+
+Lemma tm9: halts_at_trans (TM_from_str "1RB2LA1RA_1LB1LA2RC_---1LA2RB") c0 (C,0).
+Proof. solve_halt. Time Qed.
+
+Lemma tm10: halts_at_trans (TM_from_str "1RB2LA1RA_1LB1LA1RC_---2LA2RB") c0 (C,0).
+Proof. solve_halt. Time Qed.
+
+Lemma tm11: halts_at_trans (TM_from_str "1RB2LA---_0LC2RB1LB_1RA1LC2LC") c0 (A,2).
+Proof. solve_halt. Time Qed.
+
+Lemma tm12: halts_at_trans (TM_from_str "1RB1LA---_0LC2RB1LB_1RA1LC2LC") c0 (A,2).
+Proof. solve_halt. Time Qed.
+
+Lemma tm13: halts_at_trans (TM_from_str "1RB2RA1LA_0RC1RC2LA_2LC1RB---") c0 (C,2).
+Proof. solve_halt. Time Qed.
+
+Lemma tm14: halts_at_trans (TM_from_str "1RB---2LC_1LC2RB1LB_1LA2RC2LA") c0 (A,1).
+Proof. solve_halt. Time Qed.
+
+Lemma tm15: halts_at_trans (TM_from_str "1RB---2RB_1LC0LB1RA_1RA2LC1RC") c0 (A,1).
+Proof. solve_halt. Time Qed.
+
+Lemma tm16: halts_at_trans (TM_from_str "1RB2RA2RC_1LC---1LA_1RA2LB1LC") c0 (B,1).
+Proof. solve_halt. Time Qed.
+
+Lemma tm17: halts_at_trans (TM_from_str "1RB---2LC_1LC2RB1LB_1LA0RB2LA") c0 (A,1).
+Proof. solve_halt. Time Qed.
+
+Lemma tm18: halts_at_trans (TM_from_str "1RB2LA1RA_1LC1LA2RC_---1LA2RB") c0 (C,0).
+Proof. solve_halt. Time Qed.
+
+Lemma tm19: halts_at_trans (TM_from_str "1RB2LA1RA_1LC2RB1RC_---1LA1LB") c0 (C,0).
+Proof. solve_halt. Time Qed.
+
+Lemma tm20: halts_at_trans (TM_from_str "1RB2LA1RA_1RC2RB0RC_1LA---1LA") c0 (C,1).
+Proof. solve_halt. Time Qed.
+
+Lemma tm21: halts_at_trans (TM_from_str "1RB2RA1LA_2LC0RC1RB_---2LA1RB") c0 (C,0).
+Proof. solve_halt. Time Qed.
+
+Lemma tm22: halts_at_trans (TM_from_str "1RB1LA2LA_2RC1RC---_1LA2RC1LC") c0 (B,2).
+Proof. solve_halt. Time Qed.
+
+Lemma tm23: halts_at_trans (TM_from_str "1RB0LA1LA_2RC1RC---_2LC1RA0RC") c0 (B,2).
+Proof. solve_halt. Time Qed.
+
