verify/TC33.v
@@ -1,0 +1,11 @@
+Require Export String.
+Require Export NArith.
+From BusyCoq Require Export Individual33.
+From BusyCoq Require Export TC.
+
+Module TC33 := TC BB33.
+Export TC33.
+
+Open Scope string.
+
+
